Lp2lc/Active/STLC/Tests/Sanity.lean
@@ -2,16 +2,17 @@ import «Lp2lc».Active.STLC.Proof
 
 namespace Lp2lc.Active.STLC.Tests
 
+open Lp2lc.Active.STLC
+
 namespace Trm
 
-
-def trm1 (Index : Type) : _Trm Index :=
- sorry
+def trm1 (Index : Type) : Trm Index :=
+ .literal ""
 
 def trm2 : ClosedTrm :=
  trm1
 
-def trm3 (Index : Type) : _Trm Index :=
+def trm3 (Index : Type) : Trm Index :=
  trm2 Index
 
 end Trm
